# Logique de Hoare

## Règles

* {&phi;[exp/x]} x := {&phi;}


```
inst =
  si y < z (c1)
    alors m := x (inst1)
  sinon (inst 2)
    si x < z (c2)
      alors m := x (inst 2.1)
    sinon
     m := z (inst 2.2)
```

&phi;1 = {x < y}  
&phi;2 = {m = min(x, y, z)}  
Pour montrer que &phi;1 inst &ĥi;2  
Il faut montrer :
* {&phi;1 &and; &phi;2} inst1 {&phi;2} (1)
* {&phi;1 &and; &not;&phi;2} inst2 {&phi;2} (2)

### Montrons (1)
{x < y &and; y < z} m := x {m &le; x, m &le; y, m &le; z}  
* Règle n°1  
  &rarr; {&phi;2[x/m]} m := x {(&phi;2 = m &le; x, m &le; y, m &le; z)}
  &arr;  {x &le; x, x &le; y, x &le; z} (on peut supprimer x &le; x car toujours vrai)
* {x < y &and; y < z} &rArr; {x &le; y &and; y &le; z}
  + Règle n°3 &rArr; (1) OK

### Montrons (2)
(2.1) {&phi;1 &and; &not;c1 &and; c2} inst2.1 {&phi;2} idem (1)
(2.2) {&phi;1 &and; &not;c1 &and; &not;c2} inst2.2 {&phi;2} idem (1)